$$ L(w_0,w_1,\dots) = -\frac{1}{N}\sum_i \log(\sigma(y^{(i)} g(x^{(i)})) + \frac{1}{C}\sum_jw_j^2 =\\= \frac{1}{N}\sum_i \log(1+e^{-y^{(i)} \sum\limits_j w_j x_j^{(i)} }) + \frac{1}{C}\sum_jw_j^2 \\ \frac{\partial L}{\partial w_k} = -\frac{1}{N} \sum_i \frac{e^{-y^{(i)} \sum\limits_j w_j x_j^{(i)}} y^{(i)} \sum\limits_j \frac{\partial w_j}{\partial w_k} x_j^{(i)}}{1 + e^{-y^{(i)} \sum\limits_j w_j x_j^{(i)} }} + \frac{1}{C}\sum_j 2 w_j \frac{\partial w_j}{\partial w_k} = \\ = -\frac{1}{N} \sum_i \frac{y^{(i)} \sum\limits_j \delta_{jk} x_j^{(i)}}{e^{y^{(i)} \sum\limits_j w_j x_j^{(i)}} + 1} + \frac{1}{C}\sum_j 2 w_j \delta_{jk} = -\frac{1}{N} \sum_i \frac{y^{(i)} x_k^{(i)}} {e^{y^{(i)} \sum\limits_j w_j x_j^{(i)}} + 1} + \frac{2w_k}{C} = -\frac{1}{N} \sum_i y^{(i)} x_k^{(i)}\sigma(-y^{(i)} g(x^{(i)})) + \frac{2w_k}{C}$$
